src/finset_tactic.lean
@@ -3,16 +3,26 @@ import data.fintype.basic
 import extensionality
 
 namespace extensionality
-instance finset_extensionality (T : Type) [fintype T] [decidable_eq T] :
-  (boolean_algebra_extensionality (finset T) T) :=
+instance finset_ext_lemmas (T : Type) [decidable_eq T] :
+  (boolalg_ext_lemmas (finset T) T) :=
 {
   simpl_eq := by tidy,
-  ext_top := by unfold_projs; finish,
   ext_bot := by tidy,
   ext_sdiff := by tidy,
   ext_le := by tidy, 
   ext_meet := by tidy,
   ext_join := by simp only [finset.inf_eq_inter, forall_const, iff_self, finset.mem_inter, forall_true_iff],
-  ext_compl := by apply finset.mem_compl,
+}
+
+instance finset_ext_lemmas_compl (T : Type) [fintype T] [decidable_eq T] :
+  (boolalg_ext_lemmas_compl (finset T) T) :=
+{
+  ext_compl := by apply finset.mem_compl
+}
+
+instance finset_ext_lemmas_top (T : Type) [fintype T] [decidable_eq T] :
+  (boolalg_ext_lemmas_top (finset T) T) :=
+{
+  ext_top := by unfold_projs; finish,
 }
 end extensionality
